create done, delete in progress

examples/fs/FSTypes.s.dfy
@@ -25,6 +25,7 @@ module FSTypes {
   // metadata tracked by filesys
   datatype MetaData = MetaData(
     nlink: int,       // number of hard links
+    paths: seq<Path>, // paths that are hardlinked to this metadata
     size: int,        // size of file
     ftype: FileType,  // type of file
     perm: int,        // permission
@@ -35,21 +36,22 @@ module FSTypes {
     ctime: Time       // last status change time
   )
 
-  predicate ValidNewMetaData(m: MetaData)
+  predicate ValidNewMetaData(m: MetaData, path: Path)
   {
     && m.atime == m.ctime == m.mtime
     && m.size == 0
     && m.nlink == 1
+    && m.paths == [path]
   }
 
   function EmptyMetaData(): MetaData
   {
-    MetaData(0, 0, File, 0, 0, 0, Time(0,0), Time(0,0), Time(0,0))
+    MetaData(0, [], 0, File, 0, 0, 0, Time(0,0), Time(0,0), Time(0,0))
   }
 
   function InitRootMetaData(): MetaData
   {
-    MetaData(1, 0, Directory, 755, 0, 0, Time(0,0), Time(0,0), Time(0,0))
+    MetaData(1, [RootDir], 0, Directory, 755, 0, 0, Time(0,0), Time(0,0), Time(0,0))
   }
 
   function EmptyData(): Data
